theories/Events/MapDefault.v
@@ -1,0 +1,78 @@
+(** * Mutable map whose lookup operation provides a default value.*)
+
+(* begin hide *)
+Set Implicit Arguments.
+Set Contextual Implicit.
+
+From ExtLib Require Import
+     Core.RelDec.
+
+From ExtLib.Structures Require
+     Functor Monoid Maps.
+
+From ITree Require Import
+     Basics.Basics
+     Basics.CategoryOps
+     Core.ITreeDefinition
+     Indexed.Sum
+     Core.Subevent
+     Interp.Interp
+     Events.State.
+
+Import ITree.Basics.Basics.Monads.
+(* end hide *)
+
+Section Map.
+
+  Variables (K V : Type).
+
+  Variant mapE (d:V) : Type -> Type :=
+  | Insert : K -> V -> mapE d unit
+  | LookupDef : K -> mapE d V
+  | Remove : K -> mapE d unit
+  .
+
+  Arguments Insert {d}.
+  Arguments LookupDef {d}.
+  Arguments Remove {d}.
+  
+  Definition insert {E d} `{(mapE d) -< E} : K -> V -> itree E unit := embed Insert.
+  Definition lookup_def {E d} `{(mapE d) -< E} : K -> itree E V := embed LookupDef.
+  Definition remove {E d} `{(mapE d) -< E} : K -> itree E unit := embed Remove.
+
+  Import Structures.Maps.
+
+  Context {map : Type}.
+  Context {M : Map K V map}.
+
+  Definition lookup_default {K V} `{Map K V} k d m :=
+    match Maps.lookup k m with
+    | Some v' => v'
+    | None => d
+    end.
+  
+  Definition handle_map {E d} : mapE d ~> stateT map (itree E) :=
+    fun _ e env =>
+      match e with
+      | Insert k v => Ret (Maps.add k v env, tt)
+      | LookupDef k => Ret (env, lookup_default k d env)
+      | Remove k => Ret (Maps.remove k env, tt)
+      end.
+
+  Definition run_map {E d} : itree (mapE d +' E) ~> stateT map (itree E) :=
+    interp_state (case_ handle_map pure_state).
+
+
+  (* The appropriate notation of the equivalence on the state associated with
+     the MapDefault effects.  Two maps are  *)
+  Definition eq_map (d:V) (m1 m2 : map) : Prop :=
+    forall k, lookup_default k d m1 = lookup_default k d m2.
+  
+End Map.
+
+Arguments mapE {K V} d.
+Arguments insert {K V E _}.
+Arguments lookup_def {K V E _}.
+Arguments remove {K V E _}.
+Arguments run_map {K V map M _ _} [T].
+Arguments eq_map {K V map M}.
