theories/Events/MapDefaultFacts.v
@@ -1,0 +1,127 @@
+(** * Mutable map whose lookup operation provides a default value.*)
+
+(* begin hide *)
+Set Implicit Arguments.
+Set Contextual Implicit.
+
+From Coq Require Import
+     Morphisms
+     Setoid
+     RelationClasses.
+
+From ExtLib Require Import
+     Core.RelDec.
+
+From ExtLib.Structures Require
+     Functor Monoid Maps.
+
+From Paco Require Import paco.
+
+From ITree Require Import
+     Basics.Basics
+     Basics.CategoryOps
+     ITree
+     ITreeFacts
+     Indexed.Sum
+     Interp.Interp
+     Events.State
+     Events.StateFacts
+     Events.MapDefault.
+
+Import ITree.Basics.Basics.Monads.
+Import Structures.Maps.
+(* end hide *)
+
+Section MapFacts.
+
+  Variables (K V : Type).
+  Context {map : Type}.
+  Context {M : Map K V map}.
+
+  Global Instance eq_map_refl {d} : Reflexive (eq_map d).
+  Proof.
+    red. intros. unfold eq_map. tauto.
+  Qed.    
+
+  Global Instance eq_map_sym {d} : Symmetric (eq_map d).
+  Proof.
+    repeat intro.
+    unfold eq_map in H.
+    rewrite H.
+    reflexivity.
+  Qed.
+
+  Global Instance eq_map_trans {d} : Transitive (eq_map d).
+  Proof.
+    repeat intro. 
+    unfold eq_map in *.
+    rewrite H. rewrite H0. reflexivity.
+  Qed.
+
+
+  Section Relations.
+  Context {R1 R2 : Type}.
+  Variable RR : R1 -> R2 -> Prop.
+
+  Definition map_default_eq d {E} 
+    : (stateT map (itree E) R1) -> (stateT map (itree E) R2) -> Prop :=
+    fun t1 t2 => forall s1 s2, eq_map d s1 s2 -> eutt (prod_rel (eq_map d) RR) (t1 s1) (t2 s2).
+
+  End Relations.
+
+  Lemma eq_map_add:
+    forall (d : V) (s1 s2 : map) (k : K) (v : V), eq_map d s1 s2 -> eq_map d (add k v s1) (add k v s2).
+  Proof.
+    intros d s1 s2 k v H.
+    unfold eq_map in *.
+    intros.
+    unfold lookup_default in *.
+  Admitted.
+
+  Lemma eq_map_remove:
+    forall (d : V) (s1 s2 : map) (k : K), eq_map d s1 s2 -> eq_map d (remove k s1) (remove k s2).
+  Proof.
+    intros d s1 s2 k H.
+  Admitted.
+
+  
+  Lemma handle_map_eq : 
+    forall d E X (s1 s2 : map) (m : mapE d X),
+      eq_map d s1 s2 ->
+      eq_itree (prod_rel (eq_map d) eq) (handle_map m s1) ((handle_map m s2) : itree E (map * X)).
+  Proof.
+    intros.
+    destruct m; cbn; red; apply eqit_Ret; constructor; auto.
+    - apply eq_map_add. assumption.
+    - apply eq_map_remove. assumption.
+  Qed.
+
+  (* This lemma states that the operations provided by [handle_map] respect
+     the equivalence on the underlying map interface *)
+  Lemma run_map_id d {E X} (t : itree (mapE d +' E) X) :
+    map_default_eq eq d (run_map t) (run_map t).
+  Proof.
+    unfold map_default_eq, run_map; intros.
+    revert t s1 s2 H.
+    ginit.
+    gcofix CH.
+    intros.
+    repeat rewrite unfold_interp_state. unfold _interp_state.
+    destruct (observe t).
+    - gstep. constructor. constructor; auto.
+    - gstep. constructor. gbase. apply CH. assumption.
+    - gstep. constructor.
+      guclo eqit_clo_bind. econstructor.
+      unfold pure_state.
+      destruct e.
+      + cbn. eapply eqit_mon. 4 : { apply handle_map_eq. assumption. }
+        auto. auto. intros.  apply PR.
+      + cbn. apply eqit_Vis. intros.  apply eqit_Ret. constructor; auto.
+      + intros. destruct u1. destruct u2. cbn.
+        inversion H. subst.
+        gbase. apply CH. assumption.
+  Qed.
+
+
+  
+End MapFacts.
